test/norm_fin.lean
@@ -26,15 +26,15 @@ example : fin.cast_succ (fin.cast_succ (3 : fin 5)) = 10 := by norm_num
 example : equiv.swap (0 : fin 3) 1 (fin.succ 1) = 2 :=
 begin
   success_if_fail {guard_target ((equiv.swap (0 : fin 3) 1) 2 = 2)},
-  norm_num,
+  norm_fin,
   guard_target (equiv.swap (0 : fin 3) 1 2 = 2),
-  exact equiv.swap_apply_of_ne_of_ne (by dec_trivial) (by dec_trivial)
+  exact equiv.swap_apply_of_ne_of_ne dec_trivial dec_trivial
 end
 example : equiv.swap (0 : fin (1 + 2)) (1 : fin (nat.succ (1 + 1))) (fin.succ 1) = 2 :=
 begin
   success_if_fail {guard_target ((equiv.swap (0 : fin 3) 1) 2 = 2)},
-  norm_num,
+  norm_fin,
   guard_target' (equiv.swap (0 : fin 3) 1 2 = 2),
-  exact equiv.swap_apply_of_ne_of_ne (by dec_trivial) (by dec_trivial)
+  exact equiv.swap_apply_of_ne_of_ne dec_trivial dec_trivial
 end
-example : equiv.swap (0 : fin 3) 1 (fin.cast_succ 1) = 0 := by norm_num
+example : equiv.swap (0 : fin 3) 1 (fin.cast_succ 1) = 0 := by norm_fin
